\documentclass{article}
\usepackage{settings}

\geometry{
a4paper,
total={140mm,257mm},
left=35mm,
top=20mm,
}

\title{Complex Variables}
\author{Samuel Lindskog}

\begin{document}
\maketitle
\addtocontents{toc}{\protect\hypertarget{toc}{}}
\tableofcontents
\pagenumbering{gobble}
\clearpage
\pagenumbering{arabic}
\setcounter{page}{1}
\section{Complex numbers}
\subsection{Fundamental definitions and identities}
\begin{definition}[Complex number]
	A complex number is an expression with of the form \(z=x+iy\), where \(x\) and \(y\) are real numbers.
\end{definition}
\begin{definition}
	Ever complex number \(z\neq 0\) has a multiplicative inverse given by
	\begin{equation*}
		\frac{1}{z}=\frac{x-iy}{x^2+y^2}.
	\end{equation*}
\end{definition}
\begin{definition}[Modulus]
	The modulus of a complex number \(z=x+iy\) is the length of the vector \((x,y)\), and is denoted \(\abs{z}\).
	\begin{equation*}
		\abs{z}=\sqrt{x^2+y^2}.
	\end{equation*}
\end{definition}
\begin{proposition}
	For \(z,w\in\mathbb{C}\), it follows from the triangle inequality that
	\begin{IEEEeqnarray*}{l}
		\abs{z+w}\leq\abs{z}+\abs{w}\\
		\abs{z-w}\geq\abs{z}-\abs{w}
	\end{IEEEeqnarray*}
\end{proposition}
\begin{definition}[Multiplication]
	\((x+iy)(u+iv)=xu-yv+i(xv+yu)\).
\end{definition}
\begin{definition}[Complex conjugate]
	The complex conjugate of a complex number \(z=x+iy\) is defined to be \(\overbar{z}=x-iy\).
\end{definition}
\begin{proposition}
	For \(z,w\in\mathbb{C}\), the following identities hold:
	\begin{IEEEeqnarray*}{l}
	\overbar{\overbar{z}}=z\\
		\overbar{z+w}=\overbar{z}+\overbar{w}\\
		\overbar{zw}=\overbar{z}\overbar{w}\\
		\overbar{z\overbar{w}}=\overbar{z}w\\
		\abs{z}=\abs{\overbar{z}}\\
		\abs{z}^2=z\overbar{z}\\
		\abs{zw}=\abs{z}\abs{w}
	\end{IEEEeqnarray*}
\end{proposition}
\begin{proposition}
	The real and imaginary parts of \(z\) can recovered from \(z\) by
	\begin{IEEEeqnarray*}{l}
		\text{Re}\,z=(z+\overbar{z})/2\\
		\text{Im}\,z=(z-\overbar{z})/2i
	\end{IEEEeqnarray*}
\end{proposition}
\begin{lemma}[Triangle inequality in \(\mathbb{R}^n\)]
	Suppose \(a,b\in\mathbb{R}^n\), with \(\abs{a}\) the distance from \(a\) to \(0\) under the euclidean metric. Then
	\begin{equation*}
		\abs{a+b}\leq\abs{a}+\abs{b}.
	\end{equation*}
	\begin{IEEEproof}
		If dot product of two vectors is zero, they are LI. Prove basis exists such that each vector dotted with all vectors in basis is zero (use nullity potentially). if \(a,b\) vectors such that \(b\cdot a=0\), then \(a\cdot(a+b)=a\cdot a\). If \(\abs{a+b}<a\) then \(a\cdot(a+b)<a\cdot a\), so \(\abs{a+b}\geq\abs{a}\). \(\abs{a},\abs{b}\) are both geq than magnitude of their sides made of a scalar multiple of \(a+b\).
	\end{IEEEproof}
\end{lemma}
\begin{proposition}
	\label{modsquared}
	Let \(a,b\in{\mathbb{C}}\). Then
	\begin{equation*}
		\abs{a+b}^2=\abs{a}^2+\abs{b}^2+a\overline{b}+b\overline{a}=\abs{a}^2+\abs{b}^2+2\text{Re}\,a\overline{b}.
	\end{equation*}
\end{proposition}
\begin{lemma}[Triangle inequality in \(\mathbb{C}\)]
	For \(x,y\in\mathbb{C}\), \(\abs{x+y}\leq\abs{x}+\abs{y}\).
	\begin{IEEEproof}
		Suppose \(u,v\in\mathbb{R}\). Then
		\begin{IEEEeqnarray*}{l}
			\abs{u+iv}=\sqrt{u^2+v^2}\geq\sqrt{u^2}=\abs{u}\geq u.
		\end{IEEEeqnarray*}
		Therefore \(\text{Re}\,x+y\leq\abs{x+y}\) and
		\begin{IEEEeqnarray*}{l}
			2\text{Re}\,x\overbar{y}\leq2\abs{x\overbar{y}}=2\abs{xy}=2\abs{x}\abs{y}
		\end{IEEEeqnarray*}
		Because \((\abs{x}+\abs{y})^2=\abs{x}^2+\abs{y}^2+2\abs{x}\abs{y}\), it follows from proposition \ref{modsquared} that \((\abs{x}+\abs{y})^2\leq(\abs{x}+\abs{y})^2\), and therefore \(\abs{x+y}\leq\abs{x}+\abs{y}\).
	\end{IEEEproof}
\end{lemma}
\begin{definition}[Cauchy's inequality]
	\begin{equation*}
		\bigg\lvert\sum_{i=1}^{n}a_ib_i\bigg\rvert^2\leq\sum_{i=1}^n\abs{a_i}^2+\sum_{i=1}^n\abs{b_i}^2
	\end{equation*}
\end{definition}
\subsection{Polar representation}
\begin{definition}[Polar representation]
	The polar representation of a complex number \(z=x+iy\) is
	\begin{equation*}
		re^{i\theta}=r(\cos \theta+i\sin \theta).
	\end{equation*}
	Here \(r=\abs{z}\). The \emph{argument} of \(z\) is a multivalued function of \(\theta\), with
	\begin{equation*}
		\text{arg}\,z\in\{\theta+2\pi k\,|\,k\in\mathbb{Z}\}.
	\end{equation*}
	The principle value of \(\text{arg}\,z\) denoted \(\text{Arg}\,z\) is the unique member of \(\text{arg}\,z\) such that \(-\pi<\text{Arg}\,z\leq\pi\).
\end{definition}
\begin{definition}[de Moiver's formulae]
	The identies obtained by equating the imaginary and real parts of the expansions of \(e^{in\theta}\) and \((e^{in})^\theta\) are known as de Moivre's formulae, e.g.
	\begin{IEEEeqnarray*}{l}
		e^{2i\theta}=(e^{i\theta})^2\\
		\cos 2\theta+i\sin 2\theta=\cos^2 \theta+2i\cos \theta\sin \theta-\sin^2 \theta\\
		\cos 2\theta=\cos^2 \theta-\sin^2 \theta\\
		\sin 2\theta=2\cos\theta\sin \theta
	\end{IEEEeqnarray*}
\end{definition}
\begin{definition}[\(n\)th root]
	A number \(z\in\mathbb{C}\) is the \(n\)th root of \(w\in\mathbb{C}\) if \(z^n=w\). If \(w=\rho e^{i\varphi}\neq 0\), then the \(n\)th roots of \(w\) are
	\begin{equation*}
		\rho^{1/n}e^{i\varphi/n+2\pi k/n},\quad k=0,1,\ldots,n-1.
	\end{equation*}
	This is equivalent to multiplying \(\rho^{1/n}e^{i\varphi/n}\) by the \(n\)th roots of unity, i.e. all \(n\)th roots of \(1\).
\end{definition}
\subsection{Exp, log, and power functions}
\begin{definition}[Extended complex plane]
	The extended complex plane is the complex plane together with the point at infinity, denoted \(\mathbb{C}^*=\mathbb{C}\cup\{\infty\}\).
\end{definition}
\begin{proposition}
	If \(z\in\mathbb{C}\) with \(z=x+iy\) then
	\begin{equation*}
		e^z=e^xe^{iy}=e^{x}(\cos y+i\sin y).
	\end{equation*}
\end{proposition}
\section{Analytic Functions}
\subsection{Limits}
\begin{definition}[Limits]
	If the limit of \(f(z)\) as \(z\) approaches \(z_0\) is \(w_0\), this means that for all \(\epsilon\in\mathbb{R}^+\), there exists \(\delta\in\mathbb{R}^+\) such that
	\begin{equation*}
		0<\abs{z-z_0}<\delta\Rightarrow \abs{f(z)-w_0}<\epsilon.
	\end{equation*}
	This is written as \(\lim_{z\rightarrow z_0}f(z)=w_0\). If the domain or range of the function we are taking the limit of is \(\mathbb{R}^n\), the definition remains the same and uses the euclidean metric.
\end{definition}
\begin{lemma}
	The limit of a function is unique.
	\begin{IEEEproof}
		Suppose \(f:\mathbb{C}\rightarrow\mathbb{C}\) a function and that \(\lim_{z\rightarrow z_0}f(z)=w_0\) and \(\lim_{z\rightarrow z_0}f(z)=w_1\) with \(w_0\neq w_1\). Because \(w_0\neq w_1\), \(\abs{w_0-w_1}=L>0\). If we take \(\epsilon=L/2\), there exists \(\delta>0\) such that \(\abs{z-z_0}<\delta\Rightarrow \abs{f(z)-w_0}<L/2\,\wedge\,\abs{f(z)-w_1}<L/2\). Because \((z-w_1)+(w_0-z)=w_0-w_1\), by the triangle inequality \(\abs{w_0-w_1}\leq\abs{f(z)-w_0}+\abs{f(z)-w_1}=L\), a contradiction.
	\end{IEEEproof}
\end{lemma}
\clearpage
\begin{theorem}
	Suppose \(f(z)=u(x,y)+iv(x,y),\;z=x+iy\), and that \(z_0=x_0+iy_0\) and \(w_0=u_0+iv_0\). Then \(\lim_{z\rightarrow z_0}f(z)=w_0\) iff
	\begin{equation}
		\label{limreim}
		\lim_{(x,y)\rightarrow (x_0,y_0)}u(x,y)=u_0\text{ and }
		\lim_{(x,y)\rightarrow (x_0,y_0)}v(x,y)=v_0.
	\end{equation}
	\noindent\begin{IEEEproof}
		Suppose \(\lim_{z\rightarrow z_0}f(z)=w_0\). Then for all \(\epsilon>0\) there exists \(\delta>0\) such that
		\begin{IEEEeqnarray*}{l}
			\abs{(x-x_0)+i(y-y_0)}=\sqrt{(x-x_0)^2+(y-y_0)^2}<\delta\Rightarrow\\
			\abs{u(x,y)-u_0+i(v(x,y)-v_0)}=\sqrt{(u(x,y)-u_0)^2+(v(x,y)-v_0)^2}<\epsilon.
		\end{IEEEeqnarray*}
		Because \(\sqrt{(u(x,y)-u_0)^2}\leq\sqrt{(u(x,y)-u_0)^2+(v(x,y)+v_0)^2}\),
		\begin{equation*}
			\sqrt{(x-x_0)^2+(y-y_0)^2}<\delta\Rightarrow\sqrt{(u(x,y)-u_0)^2}<\epsilon.
		\end{equation*}
		Therefore wlog \(\lim_{(x,y)\rightarrow(x_0,y_0)}u(x,y)=u_0\) and \(\lim_{(x,y)\rightarrow(x_0,y_0)}v(x,y)=v_0\).
		\medbreak
		\noindent Suppose \(\lim_{(x,y)\rightarrow(x_0,y_0)}u(x,y)=u_0\) and \(\lim_{(x,y)\rightarrow(x_0,y_0)}v(x,y)=v_0\). Then for all \(\epsilon>0\) there exists \(\delta_1,\delta_2>0\) such that
		\begin{IEEEeqnarray*}{l}
			\sqrt{(x-x_0)^2+(y-y_0)^2}<\delta_1\Rightarrow\sqrt{(u(x,y)-u_0)^2}<\epsilon/2,\\
			\sqrt{(x-x_0)^2+(y-y_0)^2}<\delta_1\Rightarrow\sqrt{(v(x,y)-v_0)^2}<\epsilon/2.
		\end{IEEEeqnarray*}
		If \(0<\delta<\delta_1,\delta_2\), it follows from the triangle inequality, the definition of \(f\), and the definition of modulus that
		\begin{equation*}
			\abs{z-z_0}<\delta\Rightarrow\abs{f(z)-w_0}<\epsilon.
		\end{equation*}
		Thus \(\lim_{z\rightarrow z_0}f(z)=w_0\).
	\end{IEEEproof}
\end{theorem}
\begin{remark}
	Going forward, for \(x,y\in\mathbb{R}^n\), \(d(x,y)\) refers to the euclidean metric.
\end{remark}
\begin{theorem}
	Suppose that
	\begin{equation*}
		\lim_{z\rightarrow z_0}f(x)=w_0\text{ and }\lim_{z\rightarrow z_0}F(z)=W_0.
	\end{equation*}
	Then the following is true:
	\begin{IEEEeqnarray*}{l}
		\lim_{z\rightarrow z_0}[f(z)+F(z)]=w_0+W_0,\\
		\lim_{z\rightarrow z_0}[f(z)F(z)]=w_0W_0,\\
		\lim_{z\rightarrow z_0}\frac{f(z)}{F(z)}=\frac{w_0}{W_0},\quad W_0\neq 0.
	\end{IEEEeqnarray*}
	\begin{IEEEproof}
		prove dis
	\end{IEEEproof}
\end{theorem}
\end{document}
